More porting

src/test.lean
@@ -1,10 +1,27 @@
-import tactic.ext
+import verification.vars
 
 section
-variable (α : Type)
+parameter (R : Type)
 
-@[ext]
-structure TestStruct :=
-(x : α)
+open Types (nn rr)
 
+
+@[reducible]
+def ExprVal : Types → Type
+| nn := ℕ
+| rr := R
+
+def IdentVal : Types → Type := sorry
+def IdentVal.get : ∀ {b : Types}, IdentVal b → ℕ → ExprVal b := sorry
+
+inductive Expr : Types → Type
+| lit {b} : ExprVal b → Expr b
+| ident {b} : Ident b → Expr b
+| access {b} : Ident b → Expr nn → Expr b
+
+
+def Expr.eval (ctx : Context IdentVal) : ∀ {b}, Expr b → ExprVal b
+| _ (Expr.lit r) := r
+| b (Expr.ident x) := (λ a : Ident b → IdentVal b, IdentVal.get (a x) 0) (Context.get ctx)
+| b (Expr.access x i) := IdentVal.get (ctx.get x) i.eval --(λ a : Ident b → IdentVal b, (a x).get i') (Context.get ctx)
 end
